src/fstar/FStarC.Main.fst
@@ -259,7 +259,9 @@ let go_normal () =
 
       | Some (deps, tcr) ->
         print1 "Deps: %s\n" (show deps);
-        print1 "%s\n" (show tcr.checked_module)
+        print1 "%s\n" (show tcr.checked_module);
+        print1 "%s\n" (show <| fst tcr.smt_decls);
+        print1 "%s\n" (show <| snd tcr.smt_decls)
     )
 
     (* --read_krml_file: read and print a krml file *)
