tests/vale/X64.Vale.Decls.fst
@@ -25,7 +25,8 @@ module P = X64.Print_s
 #reset-options "--z3smtopt '(set-option :smt.arith.nl true)' --using_facts_from Prims --using_facts_from FStar.Math"
 let lemma_mul_nat (x:nat) (y:nat) : Lemma (ensures 0 <= (x `op_Multiply` y)) = ()
 #reset-options "--fuel 2 --initial_ifuel 1 --z3rlimit_factor 10 --retry 5 --query_stats"
-#set-options "--z3smtopt '(set-option :smt.qi.eager_threshold 20)'"
+#set-options "--z3smtopt '(set-option :smt.qi.eager_threshold 20)' --z3version 4.15.1"
+#restart-solver
 let cf = Lemmas_i.cf
 let ins = S.ins
 type ocmp = S.ocmp
@@ -215,6 +216,7 @@ irreducible val va_irreducible_lemma_Add64 : va_b0:va_codes -> va_s0:va_state ->
     va_sM (va_update_flags va_sM (va_update_ok va_sM (va_update_dst_operand dst va_sM va_s0)))))))
 
 #push-options "--z3rlimit_factor 20"
+#restart-solver
 irreducible let va_irreducible_lemma_Add64 va_b0 va_s0 va_sN dst src =
   (va_reveal_opaque (va_transparent_code_Add64 dst src));
   let (va_old_s:va_state) = va_s0 in
@@ -250,6 +252,7 @@ let add_wrap_lemma (x y:UInt64.t)
   (ensures add_wrap (UInt64.v x) (UInt64.v y) == UInt64.v (S.add_mod64 x y))
   [SMTPat (S.add_mod64 x y)]
 = ()
+#restart-solver
 irreducible let va_irreducible_lemma_Add64Wrap va_b0 va_s0 va_sN dst src =
   (va_reveal_opaque (va_transparent_code_Add64Wrap dst src));
   let (va_old_s:va_state) = va_s0 in
@@ -298,6 +301,7 @@ let va_transparent_code_Adc64Wrap dst src =
 let va_code_Adc64Wrap dst src =
   (va_make_opaque (va_transparent_code_Adc64Wrap dst src))
 
+#restart-solver
 irreducible val va_irreducible_lemma_Adc64Wrap : va_b0:va_codes -> va_s0:va_state -> va_sN:va_state
   -> dst:va_dst_operand -> src:va_operand
   -> Ghost (va_codes & va_state)
@@ -313,6 +317,7 @@ irreducible val va_irreducible_lemma_Adc64Wrap : va_b0:va_codes -> va_s0:va_stat
     (va_update_ok va_sM (va_update_dst_operand dst va_sM va_s0)))))))
 
 #push-options "--z3rlimit_factor 20"
+#restart-solver
 irreducible let va_irreducible_lemma_Adc64Wrap va_b0 va_s0 va_sN dst src =
   (va_reveal_opaque (va_transparent_code_Adc64Wrap dst src));
   let (va_old_s:va_state) = va_s0 in
@@ -350,6 +355,7 @@ irreducible val va_irreducible_lemma_Sub64 : va_b0:va_codes -> va_s0:va_state ->
     ((va_eval_dst_operand_uint64 va_s0 dst) - (va_eval_operand_uint64 va_s0 src))) /\ (va_state_eq
     va_sM (va_update_flags va_sM (va_update_ok va_sM (va_update_dst_operand dst va_sM va_s0)))))))
 #push-options "--z3rlimit_factor 4"
+#restart-solver
 #restart-solver
 irreducible let va_irreducible_lemma_Sub64 va_b0 va_s0 va_sN dst src =
   (va_reveal_opaque (va_transparent_code_Sub64 dst src));
